

Probability and Statistics: MA6.101

Tutorial 9 Solutions

Topics Covered: Random Vectors

Q1: Let $X = \begin{bmatrix} X_1 \\ X_2 \end{bmatrix}$ be a 2-dimensional random vector. The components X_1 and X_2 are independent random variables with the following properties:

- $E[X_1] = 2, \text{Var}(X_1) = 4$
- $E[X_2] = 5, \text{Var}(X_2) = 1$

Now, consider a new random vector Y defined by the linear transformation $Y = AX$, where

$$A = \begin{bmatrix} 1 & 2 \\ 3 & -1 \end{bmatrix}$$

Find the mean vector of Y and the covariance matrix of Y .

Solution:

First, we establish the mean vector (μ_X) and the covariance matrix (Σ_X) for the random vector X . The mean vector is simply the vector of the expected values of its components.

$$\mu_X = E[X] = \begin{bmatrix} E[X_1] \\ E[X_2] \end{bmatrix} = \begin{bmatrix} 2 \\ 5 \end{bmatrix}$$

The covariance matrix contains the variances of the components on its diagonal and the covariances between components on its off-diagonal. Since X_1 and X_2 are independent, their covariance is $\text{Cov}(X_1, X_2) = 0$.

$$\Sigma_X = C_X = \begin{bmatrix} \text{Var}(X_1) & \text{Cov}(X_1, X_2) \\ \text{Cov}(X_2, X_1) & \text{Var}(X_2) \end{bmatrix} = \begin{bmatrix} 4 & 0 \\ 0 & 1 \end{bmatrix}$$

(a) Find the mean of Y

For a linear transformation $Y = AX$, the mean of Y is given by $E[Y] = AE[X]$.

$$E[Y] = \mu_Y = \begin{bmatrix} 1 & 2 \\ 3 & -1 \end{bmatrix} \begin{bmatrix} 2 \\ 5 \end{bmatrix} = \begin{bmatrix} (1)(2) + (2)(5) \\ (3)(2) + (-1)(5) \end{bmatrix} = \begin{bmatrix} 12 \\ 1 \end{bmatrix}$$

(b) Find the covariance matrix of Y

For a linear transformation $Y = AX$, the covariance matrix of Y is given by $C_Y = AC_X A^T$. First, we find the transpose of A :

$$A^T = \begin{bmatrix} 1 & 3 \\ 2 & -1 \end{bmatrix}$$

Now we compute the product AC_XA^T :

$$\begin{aligned}
C_Y = \Sigma_Y &= \left(\begin{bmatrix} 1 & 2 \\ 3 & -1 \end{bmatrix} \begin{bmatrix} 4 & 0 \\ 0 & 1 \end{bmatrix} \right) \begin{bmatrix} 1 & 3 \\ 2 & -1 \end{bmatrix} \\
&= \begin{bmatrix} (1)(4) + (2)(0) & (1)(0) + (2)(1) \\ (3)(4) + (-1)(0) & (3)(0) + (-1)(1) \end{bmatrix} \begin{bmatrix} 1 & 3 \\ 2 & -1 \end{bmatrix} \\
&= \begin{bmatrix} 4 & 2 \\ 12 & -1 \end{bmatrix} \begin{bmatrix} 1 & 3 \\ 2 & -1 \end{bmatrix} \\
&= \begin{bmatrix} (4)(1) + (2)(2) & (4)(3) + (2)(-1) \\ (12)(1) + (-1)(2) & (12)(3) + (-1)(-1) \end{bmatrix} \\
&= \begin{bmatrix} 8 & 10 \\ 10 & 37 \end{bmatrix}
\end{aligned}$$

So, the mean vector of Y is $\mu_Y = \begin{bmatrix} 12 \\ 1 \end{bmatrix}$ and its covariance matrix is $\Sigma_Y = \begin{bmatrix} 8 & 10 \\ 10 & 37 \end{bmatrix}$. Notice that even though X_1 and X_2 were independent, the new components Y_1 and Y_2 are correlated ($Cov(Y_1, Y_2) = 10$).

Q2: Let X_1 be a uniform random variable with support $R_{X_1} = [1, 2]$ and probability density function

$$f_{X_1}(x_1) = \begin{cases} 1 & \text{if } x_1 \in R_{X_1} \\ 0 & \text{if } x_1 \notin R_{X_1} \end{cases}$$

Let X_2 be a continuous random variable, independent of X_1 , with support $R_{X_2} = [0, 2]$ and probability density function

$$f_{X_2}(x_2) = \begin{cases} \frac{3}{8}x_2^2 & \text{if } x_2 \in R_{X_2} \\ 0 & \text{if } x_2 \notin R_{X_2} \end{cases}$$

Let

$$\mathbf{Y} = \begin{bmatrix} Y_1 \\ Y_2 \end{bmatrix} = \begin{bmatrix} X_1^2 \\ X_1 + X_2 \end{bmatrix}$$

Find the joint probability density function of the random vector \mathbf{Y} .

Solution:

Since X_1 and X_2 are independent, their joint probability density function is the product of their marginals.

$$f_{X_1, X_2}(x_1, x_2) = f_{X_1}(x_1)f_{X_2}(x_2) = \begin{cases} \frac{3}{8}x_2^2 & \text{if } x_1 \in [1, 2] \text{ and } x_2 \in [0, 2] \\ 0 & \text{otherwise} \end{cases}$$

The transformation is $g(x) = [X_1^2, X_1 + X_2]^T$. The inverse transformation $g^{-1}(y)$ is $x_1 = \sqrt{y_1}$ and $x_2 = y_2 - \sqrt{y_1}$. The Jacobian matrix of the inverse is:

$$J_{g^{-1}}(y) = \begin{bmatrix} \frac{\partial x_1}{\partial y_1} & \frac{\partial x_1}{\partial y_2} \\ \frac{\partial x_2}{\partial y_1} & \frac{\partial x_2}{\partial y_2} \end{bmatrix} = \begin{bmatrix} \frac{1}{2\sqrt{y_1}} & 0 \\ -\frac{1}{2\sqrt{y_1}} & 1 \end{bmatrix}$$

The determinant is $\det(J_{g^{-1}}(y)) = \frac{1}{2\sqrt{y_1}}$. The formula for the transformed PDF is $f_{\mathbf{Y}}(y) = f_{\mathbf{X}}(g^{-1}(y))|\det(J_{g^{-1}}(y))|$.

$$f_{\mathbf{X}}(g^{-1}(y))|\det(J_{g^{-1}}(y))| = f_{X_1, X_2}(\sqrt{y_1}, y_2 - \sqrt{y_1}) \cdot \frac{1}{2\sqrt{y_1}} = \frac{3}{8}(y_2 - \sqrt{y_1})^2 \cdot \frac{1}{2\sqrt{y_1}} = \frac{3}{16\sqrt{y_1}}(y_2 - \sqrt{y_1})^2$$

The support for \mathbf{Y} is found from the support of \mathbf{X} : $1 \leq x_1 \leq 2 \implies 1 \leq y_1 \leq 4$. And $0 \leq x_2 \leq 2 \implies 0 \leq y_2 - \sqrt{y_1} \leq 2 \implies \sqrt{y_1} \leq y_2 \leq \sqrt{y_1} + 2$. So the final PDF is:

$$f_{\mathbf{Y}}(y_1, y_2) = \begin{cases} \frac{3}{16\sqrt{y_1}}(y_2 - \sqrt{y_1})^2 & \text{if } 1 \leq y_1 \leq 4 \text{ and } \sqrt{y_1} \leq y_2 \leq \sqrt{y_1} + 2 \\ 0 & \text{otherwise} \end{cases}$$

Q3: Let X and Y be said to be bivariate normal if $aX + bY$ is normal for all a and b . If X and Y are bivariate normal with 0 mean, variance of 1, and ρ correlation, derive their joint PDF:

$$f(x, y) = \frac{1}{2\pi\sqrt{1-\rho^2}} \exp\left(-\frac{1}{2(1-\rho^2)}(x^2 - 2\rho xy + y^2)\right)$$

Solution:

Let $\mathbf{X} = \begin{bmatrix} X \\ Y \end{bmatrix}$. The mean vector is $\mu = \begin{bmatrix} 0 \\ 0 \end{bmatrix}$. The covariance matrix is $\Sigma = \begin{bmatrix} 1 & \rho \\ \rho & 1 \end{bmatrix}$.

The determinant is $\det(\Sigma) = 1 - \rho^2$ and the inverse is $\Sigma^{-1} = \frac{1}{1-\rho^2} \begin{bmatrix} 1 & -\rho \\ -\rho & 1 \end{bmatrix}$. The multivariate normal PDF is $f(\mathbf{x}) = \frac{1}{\sqrt{(2\pi)^n \det(\Sigma)}} \exp\left(-\frac{1}{2}(\mathbf{x} - \mu)^T \Sigma^{-1}(\mathbf{x} - \mu)\right)$. The quadratic form in the exponent is:

$$(\mathbf{x} - \mu)^T \Sigma^{-1}(\mathbf{x} - \mu) = \begin{bmatrix} x & y \end{bmatrix} \frac{1}{1-\rho^2} \begin{bmatrix} 1 & -\rho \\ -\rho & 1 \end{bmatrix} \begin{bmatrix} x \\ y \end{bmatrix} = \frac{1}{1-\rho^2}(x^2 - 2\rho xy + y^2)$$

Substituting this back gives the desired formula.

Q4: Suppose $\mathbf{X} \sim \mathcal{N}(\boldsymbol{\mu}, \Sigma)$. Now consider $\mathbf{Y} = \mathbf{A}\mathbf{X} + \mathbf{b}$. Then we have

$$\mathbf{Y} \sim \mathcal{N}(\mathbf{A}E[\mathbf{X}] + \mathbf{b}, \mathbf{A}\Sigma\mathbf{A}^T).$$

Prove this using Moment-Generating Functions (MGFs).

A:

Our goal is to find the MGF of \mathbf{Y} , defined as $M_{\mathbf{Y}}(\mathbf{t}) = E[e^{\mathbf{t}^T \mathbf{Y}}]$, and show that it matches the MGF of the target normal distribution.

We are given that $\mathbf{X} \sim \mathcal{N}(\boldsymbol{\mu}, \Sigma)$, where $E[\mathbf{X}] = \boldsymbol{\mu}$. The MGF of \mathbf{X} is known to be:

$$M_{\mathbf{X}}(\mathbf{s}) = E[e^{\mathbf{s}^T \mathbf{X}}] = \exp\left(\mathbf{s}^T \boldsymbol{\mu} + \frac{1}{2} \mathbf{s}^T \Sigma \mathbf{s}\right)$$

We begin with the definition of $M_{\mathbf{Y}}(\mathbf{t})$ and substitute $\mathbf{Y} = \mathbf{A}\mathbf{X} + \mathbf{b}$:

$$\begin{aligned} M_{\mathbf{Y}}(\mathbf{t}) &= E[e^{\mathbf{t}^T \mathbf{Y}}] \\ &= E[e^{\mathbf{t}^T (\mathbf{A}\mathbf{X} + \mathbf{b})}] \\ &= E[e^{\mathbf{t}^T \mathbf{A}\mathbf{X} + \mathbf{t}^T \mathbf{b}}] \\ &= E[e^{\mathbf{t}^T \mathbf{A}\mathbf{X}} \cdot e^{\mathbf{t}^T \mathbf{b}}] \end{aligned}$$

Since $e^{\mathbf{t}^T \mathbf{b}}$ is a scalar constant with respect to the expectation, we can factor it out:

$$M_{\mathbf{Y}}(\mathbf{t}) = e^{\mathbf{t}^T \mathbf{b}} \cdot E[e^{\mathbf{t}^T \mathbf{A}\mathbf{X}}]$$

Now, we use the transpose property $(\mathbf{A}\mathbf{B})^T = \mathbf{B}^T \mathbf{A}^T$, which implies $\mathbf{t}^T \mathbf{A} = (\mathbf{A}^T \mathbf{t})^T$.

$$M_{\mathbf{Y}}(\mathbf{t}) = e^{\mathbf{t}^T \mathbf{b}} \cdot E[e^{(\mathbf{A}^T \mathbf{t})^T \mathbf{X}}]$$

We recognize the expectation term $E[e^{(\mathbf{A}^T \mathbf{t})^T \mathbf{X}}]$ as the MGF of \mathbf{X} , $M_{\mathbf{X}}(\mathbf{s})$, evaluated at the vector $\mathbf{s} = \mathbf{A}^T \mathbf{t}$.

$$M_{\mathbf{Y}}(\mathbf{t}) = e^{\mathbf{t}^T \mathbf{b}} \cdot M_{\mathbf{X}}(\mathbf{A}^T \mathbf{t})$$

Next, we substitute the known formula for $M_{\mathbf{X}}$:

$$M_{\mathbf{Y}}(\mathbf{t}) = e^{\mathbf{t}^T \mathbf{b}} \cdot \exp \left((\mathbf{A}^T \mathbf{t})^T \boldsymbol{\mu} + \frac{1}{2} (\mathbf{A}^T \mathbf{t})^T \boldsymbol{\Sigma} (\mathbf{A}^T \mathbf{t}) \right)$$

We simplify the terms in the exponent using $(\mathbf{A}^T \mathbf{t})^T = \mathbf{t}^T (\mathbf{A}^T)^T = \mathbf{t}^T \mathbf{A}$:

$$\begin{aligned} M_{\mathbf{Y}}(\mathbf{t}) &= e^{\mathbf{t}^T \mathbf{b}} \cdot \exp \left((\mathbf{t}^T \mathbf{A}) \boldsymbol{\mu} + \frac{1}{2} (\mathbf{t}^T \mathbf{A}) \boldsymbol{\Sigma} (\mathbf{A}^T \mathbf{t}) \right) \\ &= e^{\mathbf{t}^T \mathbf{b}} \cdot \exp \left(\mathbf{t}^T (\mathbf{A} \boldsymbol{\mu}) + \frac{1}{2} \mathbf{t}^T (\mathbf{A} \boldsymbol{\Sigma} \mathbf{A}^T) \mathbf{t} \right) \end{aligned}$$

Finally, we combine the terms into a single exponent:

$$\begin{aligned} M_{\mathbf{Y}}(\mathbf{t}) &= \exp \left(\mathbf{t}^T \mathbf{b} + \mathbf{t}^T (\mathbf{A} \boldsymbol{\mu}) + \frac{1}{2} \mathbf{t}^T (\mathbf{A} \boldsymbol{\Sigma} \mathbf{A}^T) \mathbf{t} \right) \\ &= \exp \left(\mathbf{t}^T (\mathbf{A} \boldsymbol{\mu} + \mathbf{b}) + \frac{1}{2} \mathbf{t}^T (\mathbf{A} \boldsymbol{\Sigma} \mathbf{A}^T) \mathbf{t} \right) \end{aligned}$$

This final expression is the MGF of a multivariate normal distribution. By the uniqueness property of MGFs, we can identify the mean and covariance matrix by comparing our result to the general form $M(\mathbf{t}) = \exp(\mathbf{t}^T \boldsymbol{\mu}_{\text{new}} + \frac{1}{2} \mathbf{t}^T \boldsymbol{\Sigma}_{\text{new}} \mathbf{t})$.

We find:

- New Mean: $\boldsymbol{\mu}_{\mathbf{Y}} = \mathbf{A} \boldsymbol{\mu} + \mathbf{b} = \mathbf{A} E[\mathbf{X}] + \mathbf{b}$
- New Covariance: $\boldsymbol{\Sigma}_{\mathbf{Y}} = \mathbf{A} \boldsymbol{\Sigma} \mathbf{A}^T$

Therefore, we have shown that $\mathbf{Y} \sim \mathcal{N}(\mathbf{A}\boldsymbol{\mu} + \mathbf{b}, \mathbf{A}\boldsymbol{\Sigma}\mathbf{A}^T)$.

Q5: Let $\mathbf{X} = [X_1, X_2]^T$ be a bivariate normal random vector with mean $\boldsymbol{\mu} = \begin{bmatrix} 0 \\ 0 \end{bmatrix}$ and covariance $\boldsymbol{\Sigma} = \begin{bmatrix} 5 & 2 \\ 2 & 1 \end{bmatrix}$. Find a constant a such that the random variables $Y_1 = X_1 + aX_2$ and $Y_2 = X_2$ are independent.

Solution:

For jointly normal random variables, independence is equivalent to being uncorrelated. So, we need to find the value of a that makes Y_1 and Y_2 uncorrelated, which means their covariance must be zero: $Cov(Y_1, Y_2) = 0$.

We can compute the covariance:

$$\begin{aligned} Cov(Y_1, Y_2) &= Cov(X_1 + aX_2, X_2) \\ &= Cov(X_1, X_2) + Cov(aX_2, X_2) \quad (\text{by bilinearity of covariance}) \\ &= Cov(X_1, X_2) + a \cdot Cov(X_2, X_2) \\ &= Cov(X_1, X_2) + a \cdot Var(X_2) \end{aligned}$$

From the given covariance matrix $\boldsymbol{\Sigma}$, we have $Cov(X_1, X_2) = 2$ and $Var(X_2) = 1$. Substituting these values into the equation:

$$Cov(Y_1, Y_2) = 2 + a(1)$$

To make them uncorrelated, we set the covariance to zero:

$$2 + a = 0 \implies a = -2$$

Thus, when $a = -2$, the random variables $Y_1 = X_1 - 2X_2$ and $Y_2 = X_2$ are uncorrelated, and because they are linear combinations of jointly normal variables, they are also independent.

Q6: Let $x = \begin{bmatrix} x_1 \\ x_2 \end{bmatrix}$ belong to a bivariate normal distribution $\mathcal{N}\left(\begin{bmatrix} \mu_1 \\ \mu_2 \end{bmatrix}, \begin{bmatrix} \Sigma_{11} & \Sigma_{12} \\ \Sigma_{21} & \Sigma_{22} \end{bmatrix}\right)$.

Show that $x_1|x_2 \sim \mathcal{N}(\mu_{1|2}, \Sigma_{1|2})$ where

$$\mu_{1|2} = \mu_1 + \Sigma_{12}\Sigma_{22}^{-1}(x_2 - \mu_2)$$

$$\Sigma_{1|2} = \Sigma_{11} - \Sigma_{12}\Sigma_{22}^{-1}\Sigma_{21}$$

A: The marginal distribution of x_2 is given by $\mathcal{N}(\mu_2, \Sigma_2)$. Using conditional probability

$$\begin{aligned} p(x_1|x_2) &= \frac{\mathcal{N}(x; \boldsymbol{\mu}, \boldsymbol{\Sigma})}{\mathcal{N}(x_2; \mu_2, \Sigma_{22})} \\ p(x; \boldsymbol{\mu}, \boldsymbol{\Sigma}) &= \frac{1}{2\pi\sqrt{|\boldsymbol{\Sigma}|}} \exp\left[-\frac{1}{2}(x - \boldsymbol{\mu})^T \boldsymbol{\Sigma}^{-1}(x - \boldsymbol{\mu})\right] \end{aligned}$$

$$\begin{aligned}
&= p(x_1|x_2) = \frac{1}{\sqrt{(2\pi)\Sigma_{22}}} \exp \left[-\frac{1}{2} \frac{(x_2 - \mu_2)^2}{\Sigma_{22}} \right] \\
&= \frac{1}{\sqrt{(2\pi)|\Sigma_{11}|}} \cdot \frac{\sqrt{|\Sigma_{22}|}}{\sqrt{|\Sigma|}} \exp \left[-\frac{1}{2} (x - \mu)^T \Sigma^{-1} (x - \mu) + \frac{1}{2} \frac{(x_2 - \mu_2)^2}{\Sigma_{22}} \right] \\
&= \frac{1}{\sqrt{(2\pi)|\Sigma_{11}|}} \cdot \frac{\sqrt{|\Sigma_{22}|}}{\sqrt{|\Sigma|}} \exp \left[-\frac{1}{2} \begin{bmatrix} x_1 - \mu_1 \\ x_2 - \mu_2 \end{bmatrix}^T \Sigma^{-1} \begin{bmatrix} x_1 - \mu_1 \\ x_2 - \mu_2 \end{bmatrix} + \frac{1}{2} \frac{(x_2 - \mu_2)^2}{\Sigma_{22}} \right]
\end{aligned}$$

For a 2x2 matrix $A = \begin{bmatrix} a & b \\ c & d \end{bmatrix}$ the inverse is given by

$$A^{-1} = \frac{1}{|A|} \begin{bmatrix} d & -b \\ -c & a \end{bmatrix}$$

Using this and expanding

$$\begin{aligned}
p(x_1|x_2) &= \frac{1}{\sqrt{(2\pi)|\Sigma_{11}|}} \cdot \frac{\sqrt{|\Sigma_{22}|}}{\sqrt{|\Sigma|}} \exp \left[-\frac{1}{2|\Sigma|} (\Sigma_{11}(x_2 - \mu_2)^2 \right. \\
&\quad \left. + 2\Sigma_{12}(x_2 - \mu_2)(x_1 - \mu_1) + \Sigma_{22}(x_1 - \mu_1)^2) + \frac{1}{2} \frac{(x_2 - \mu_2)^2}{\Sigma_{22}} \right] \\
&= \frac{1}{\sqrt{(2\pi)|\Sigma_{11}|}} \cdot \frac{\sqrt{|\Sigma_{22}|}}{\sqrt{|\Sigma|}} \exp \left[-\frac{1}{2|\Sigma|\Sigma_{22}} (\Sigma_{12}^2(x_2 - \mu_2)^2 \right. \\
&\quad \left. - 2\Sigma_{12}\Sigma_{22}(x_2 - \mu_2)(x_1 - \mu_1) + \Sigma_{22}^2(x_1 - \mu_1)^2) \right] \\
&= \frac{1}{\sqrt{(2\pi)|\Sigma_{11}|}} \cdot \frac{\sqrt{|\Sigma_{22}|}}{\sqrt{|\Sigma|}} \exp \left[-\frac{1}{2|\Sigma|\Sigma_{22}} (\Sigma_{22}(x_1 - \mu_1) - \Sigma_{12}(x_2 - \mu_2))^2 \right] \\
&= \frac{1}{\sqrt{(2\pi)|\Sigma_{11}|}} \cdot \frac{\sqrt{|\Sigma_{22}|}}{\sqrt{|\Sigma|}} \exp \left[-\frac{\Sigma_{22}}{2|\Sigma|} \left(x_1 - \mu_1 - \frac{\Sigma_{12}}{\Sigma_{22}}(x_2 - \mu_2) \right)^2 \right] \\
&= \frac{1}{\sqrt{(2\pi)|\Sigma_{11}|}} \cdot \frac{\sqrt{|\Sigma_{22}|}}{\sqrt{|\Sigma|}} \exp \left[-\frac{1}{2} \left(\frac{x_1 - (\mu_1 - \Sigma_{12}\Sigma_{22}^{-1}(x_2 - \mu_2))}{\sqrt{\Sigma_{11} - \Sigma_{12}\Sigma_{22}^{-1}\Sigma_{12}}} \right)^2 \right]
\end{aligned}$$

Thus the mean and variance are

$$\begin{aligned}
\mu_{1|2} &= \mu_1 + \Sigma_{12}\Sigma_{22}^{-1}(x_2 - \mu_2) \\
\Sigma_{1|2} &= \Sigma_{11} - \Sigma_{12}\Sigma_{22}^{-1}\Sigma_{21}
\end{aligned}$$

Q7: Let $\mathbf{X} \in \mathbb{R}^n$ be a random vector with mean $\mu = E[\mathbf{X}]$ and covariance matrix $\Sigma = \text{Cov}(\mathbf{X})$. Let $a, b \in \mathbb{R}^n$ be fixed (non-random) vectors.

(a) Show that

$$\text{Var}(a^T \mathbf{X}) = a^T \Sigma a, \quad \text{and} \quad \text{Cov}(a^T \mathbf{X}, b^T \mathbf{X}) = a^T \Sigma b.$$

(b) Using

$$\Sigma = \begin{bmatrix} 4 & 1 \\ 1 & 2 \end{bmatrix}, \quad a = \begin{bmatrix} 2 \\ -1 \end{bmatrix}, \quad b = \begin{bmatrix} 1 \\ 3 \end{bmatrix},$$

compute both $\text{Var}(a^T \mathbf{X})$ and $\text{Cov}(a^T \mathbf{X}, b^T \mathbf{X})$ numerically.

Solution:

(a) Detailed Proof:

We start with the definitions of variance and covariance. For any random variables Y_1, Y_2 ,

$$\text{Cov}(Y_1, Y_2) = E[(Y_1 - E[Y_1])(Y_2 - E[Y_2])].$$

Let

$$Y_1 = a^T \mathbf{X}, \quad Y_2 = b^T \mathbf{X}.$$

Then

$$E[Y_1] = a^T E[\mathbf{X}] = a^T \mu, \quad E[Y_2] = b^T E[\mathbf{X}] = b^T \mu.$$

Now,

$$\text{Cov}(a^T \mathbf{X}, b^T \mathbf{X}) = E[(a^T \mathbf{X} - a^T \mu)(b^T \mathbf{X} - b^T \mu)].$$

Simplifying,

$$\text{Cov}(a^T \mathbf{X}, b^T \mathbf{X}) = E[a^T (\mathbf{X} - \mu)(b^T (\mathbf{X} - \mu))].$$

Since $(b^T (\mathbf{X} - \mu))$ is a scalar, we can rewrite it as

$$(a^T (\mathbf{X} - \mu))(b^T (\mathbf{X} - \mu)) = a^T (\mathbf{X} - \mu)(\mathbf{X} - \mu)^T b.$$

Therefore,

$$\text{Cov}(a^T \mathbf{X}, b^T \mathbf{X}) = E[a^T (\mathbf{X} - \mu)(\mathbf{X} - \mu)^T b] = a^T E[(\mathbf{X} - \mu)(\mathbf{X} - \mu)^T] b.$$

By definition of covariance matrix, $E[(\mathbf{X} - \mu)(\mathbf{X} - \mu)^T] = \Sigma$. Hence,

$$\boxed{\text{Cov}(a^T \mathbf{X}, b^T \mathbf{X}) = a^T \Sigma b.}$$

If we take $a = b$, then this reduces to

$$\text{Var}(a^T \mathbf{X}) = a^T \Sigma a.$$

Alternative viewpoint: By the bilinearity of covariance,

$$\text{Var}(a^T \mathbf{X} + b^T \mathbf{X}) = \text{Var}(a^T \mathbf{X}) + \text{Var}(b^T \mathbf{X}) + 2 \text{Cov}(a^T \mathbf{X}, b^T \mathbf{X}),$$

and since $\text{Var}(c^T \mathbf{X}) = c^T \Sigma c$ for any c , comparing terms yields $\text{Cov}(a^T \mathbf{X}, b^T \mathbf{X}) = a^T \Sigma b$ as before.

(b) Numerical Computation:

Given

$$\Sigma = \begin{bmatrix} 4 & 1 \\ 1 & 2 \end{bmatrix}, \quad a = \begin{bmatrix} 2 \\ -1 \end{bmatrix}, \quad b = \begin{bmatrix} 1 \\ 3 \end{bmatrix}.$$

Step 1: Compute Σa and Σb .

$$\Sigma a = \begin{bmatrix} 4 & 1 \\ 1 & 2 \end{bmatrix} \begin{bmatrix} 2 \\ -1 \end{bmatrix} = \begin{bmatrix} 8 - 1 \\ 2 - 2 \end{bmatrix} = \begin{bmatrix} 7 \\ 0 \end{bmatrix}.$$

$$\Sigma b = \begin{bmatrix} 4 & 1 \\ 1 & 2 \end{bmatrix} \begin{bmatrix} 1 \\ 3 \end{bmatrix} = \begin{bmatrix} 4 + 3 \\ 1 + 6 \end{bmatrix} = \begin{bmatrix} 7 \\ 7 \end{bmatrix}.$$

Step 2: Compute $\text{Var}(a^T \mathbf{X})$ and $\text{Cov}(a^T \mathbf{X}, b^T \mathbf{X})$.

$$\text{Var}(a^T \mathbf{X}) = a^T \Sigma a = \begin{bmatrix} 2 & -1 \end{bmatrix} \begin{bmatrix} 7 \\ 0 \end{bmatrix} = 14.$$

$$\text{Cov}(a^T \mathbf{X}, b^T \mathbf{X}) = a^T \Sigma b = \begin{bmatrix} 2 & -1 \end{bmatrix} \begin{bmatrix} 7 \\ 7 \end{bmatrix} = 14 - 7 = 7.$$

Final Answers:

$$\boxed{\text{Var}(a^T \mathbf{X}) = 14, \quad \text{Cov}(a^T \mathbf{X}, b^T \mathbf{X}) = 7.}$$

Q8: Let (\mathbf{X}, \mathbf{Y}) be a jointly distributed random vector in \mathbb{R}^{n+m} , where

$$\mathbf{X} = \begin{bmatrix} X_1 \\ \vdots \\ X_n \end{bmatrix} \in \mathbb{R}^n, \quad \mathbf{Y} = \begin{bmatrix} Y_1 \\ \vdots \\ Y_m \end{bmatrix} \in \mathbb{R}^m,$$

and assume all components have finite second moments. Define the conditional mean and conditional covariance of \mathbf{Y} given \mathbf{X} as

$$\boldsymbol{\mu}_{\mathbf{Y}|\mathbf{X}} := E[\mathbf{Y} | \mathbf{X}], \quad \boldsymbol{\Sigma}_{\mathbf{Y}|\mathbf{X}} := \text{Cov}(\mathbf{Y} | \mathbf{X}) = E[(\mathbf{Y} - \boldsymbol{\mu}_{\mathbf{Y}|\mathbf{X}})(\mathbf{Y} - \boldsymbol{\mu}_{\mathbf{Y}|\mathbf{X}})^T | \mathbf{X}].$$

(a) Show that the unconditional mean of \mathbf{Y} can be expressed as

$$E[\mathbf{Y}] = E[\boldsymbol{\mu}_{\mathbf{Y}|\mathbf{X}}] = E[E[\mathbf{Y} | \mathbf{X}]].$$

(b) Prove that the covariance matrix of \mathbf{Y} satisfies

$$\text{Cov}(\mathbf{Y}) = E[\boldsymbol{\Sigma}_{\mathbf{Y}|\mathbf{X}}] + \text{Cov}(\boldsymbol{\mu}_{\mathbf{Y}|\mathbf{X}}).$$

(c) Suppose \mathbf{Y} is given by the linear model

$$\mathbf{Y} = A\mathbf{X} + \mathbf{Z},$$

where A is an $(m \times n)$ constant matrix, and \mathbf{X} and \mathbf{Z} are independent random vectors satisfying

$$E[\mathbf{X}] = \mathbf{0}, \quad \text{Cov}(\mathbf{X}) = \boldsymbol{\Sigma}_{\mathbf{X}}, \quad E[\mathbf{Z}] = \mathbf{0}, \quad \text{Cov}(\mathbf{Z}) = \boldsymbol{\Sigma}_{\mathbf{Z}}.$$

Using parts (a) and (b), derive expressions for $E[\mathbf{Y}]$ and $\text{Cov}(\mathbf{Y})$. Then compute $\text{Cov}(\mathbf{Y})$ numerically for

$$A = \begin{bmatrix} 1 & 2 \\ 0 & 1 \end{bmatrix}, \quad \boldsymbol{\Sigma}_{\mathbf{X}} = \begin{bmatrix} 4 & 1 \\ 1 & 3 \end{bmatrix}, \quad \boldsymbol{\Sigma}_{\mathbf{Z}} = \begin{bmatrix} 1 & 0 \\ 0 & 2 \end{bmatrix}.$$

Solution:

(a) By definition of conditional expectation,

$$E[\mathbf{Y}] = \int \mathbf{y} f_{\mathbf{Y}}(\mathbf{y}) d\mathbf{y} = \int E[\mathbf{Y} | \mathbf{X} = \mathbf{x}] f_{\mathbf{X}}(\mathbf{x}) d\mathbf{x} = E[E[\mathbf{Y} | \mathbf{X}]] = E[\boldsymbol{\mu}_{\mathbf{Y}|\mathbf{X}}].$$

Hence, the overall mean equals the expected conditional mean:

$$\boxed{E[\mathbf{Y}] = E[E[\mathbf{Y} \mid \mathbf{X}]]}.$$

(b) Start from the definition of covariance:

$$\text{Cov}(\mathbf{Y}) = E[(\mathbf{Y} - E[\mathbf{Y}])(\mathbf{Y} - E[\mathbf{Y}])^T].$$

Add and subtract $\boldsymbol{\mu}_{\mathbf{Y}|\mathbf{X}}$:

$$\mathbf{Y} - E[\mathbf{Y}] = (\mathbf{Y} - \boldsymbol{\mu}_{\mathbf{Y}|\mathbf{X}}) + (\boldsymbol{\mu}_{\mathbf{Y}|\mathbf{X}} - E[\mathbf{Y}]).$$

Then expand the product:

$$\begin{aligned} \text{Cov}(\mathbf{Y}) &= E[(\mathbf{Y} - \boldsymbol{\mu}_{\mathbf{Y}|\mathbf{X}})(\mathbf{Y} - \boldsymbol{\mu}_{\mathbf{Y}|\mathbf{X}})^T] \\ &\quad + E[(\mathbf{Y} - \boldsymbol{\mu}_{\mathbf{Y}|\mathbf{X}})(\boldsymbol{\mu}_{\mathbf{Y}|\mathbf{X}} - E[\mathbf{Y}])^T] \\ &\quad + E[(\boldsymbol{\mu}_{\mathbf{Y}|\mathbf{X}} - E[\mathbf{Y}])(\mathbf{Y} - \boldsymbol{\mu}_{\mathbf{Y}|\mathbf{X}})^T] \\ &\quad + E[(\boldsymbol{\mu}_{\mathbf{Y}|\mathbf{X}} - E[\mathbf{Y}])(\boldsymbol{\mu}_{\mathbf{Y}|\mathbf{X}} - E[\mathbf{Y}])^T]. \end{aligned}$$

Since $E[\mathbf{Y} - \boldsymbol{\mu}_{\mathbf{Y}|\mathbf{X}} \mid \mathbf{X}] = \mathbf{0}$, the second and third terms vanish. Thus,

$$\text{Cov}(\mathbf{Y}) = E[E[(\mathbf{Y} - \boldsymbol{\mu}_{\mathbf{Y}|\mathbf{X}})(\mathbf{Y} - \boldsymbol{\mu}_{\mathbf{Y}|\mathbf{X}})^T \mid \mathbf{X}]] + E[(\boldsymbol{\mu}_{\mathbf{Y}|\mathbf{X}} - E[\mathbf{Y}])(\boldsymbol{\mu}_{\mathbf{Y}|\mathbf{X}} - E[\mathbf{Y}])^T].$$

The first term equals $E[\boldsymbol{\Sigma}_{\mathbf{Y}|\mathbf{X}}]$ and the second equals $\text{Cov}(\boldsymbol{\mu}_{\mathbf{Y}|\mathbf{X}})$. Therefore,

$$\boxed{\text{Cov}(\mathbf{Y}) = E[\boldsymbol{\Sigma}_{\mathbf{Y}|\mathbf{X}}] + \text{Cov}(\boldsymbol{\mu}_{\mathbf{Y}|\mathbf{X}})}.$$

(c) For $\mathbf{Y} = \mathbf{A}\mathbf{X} + \mathbf{Z}$ with \mathbf{X} and \mathbf{Z} independent and zero mean:

$$E[\mathbf{Y} \mid \mathbf{X}] = \mathbf{A}\mathbf{X} + E[\mathbf{Z} \mid \mathbf{X}] = \mathbf{A}\mathbf{X}, \quad \text{Cov}(\mathbf{Y} \mid \mathbf{X}) = \text{Cov}(\mathbf{Z}) = \boldsymbol{\Sigma}_{\mathbf{Z}}.$$

By part (a),

$$E[\mathbf{Y}] = E[E[\mathbf{Y} \mid \mathbf{X}]] = \mathbf{A}E[\mathbf{X}] = \mathbf{0}.$$

By part (b),

$$\text{Cov}(\mathbf{Y}) = E[\text{Cov}(\mathbf{Y} \mid \mathbf{X})] + \text{Cov}(E[\mathbf{Y} \mid \mathbf{X}]) = \boldsymbol{\Sigma}_{\mathbf{Z}} + \text{Cov}(\mathbf{A}\mathbf{X}) = \boldsymbol{\Sigma}_{\mathbf{Z}} + \mathbf{A}\boldsymbol{\Sigma}_{\mathbf{X}}\mathbf{A}^T.$$

Numerical computation:

$$\mathbf{A} = \begin{bmatrix} 1 & 2 \\ 0 & 1 \end{bmatrix}, \quad \boldsymbol{\Sigma}_{\mathbf{X}} = \begin{bmatrix} 4 & 1 \\ 1 & 3 \end{bmatrix}, \quad \boldsymbol{\Sigma}_{\mathbf{Z}} = \begin{bmatrix} 1 & 0 \\ 0 & 2 \end{bmatrix}.$$

Compute

$$\mathbf{A}\boldsymbol{\Sigma}_{\mathbf{X}} = \begin{bmatrix} 6 & 7 \\ 1 & 3 \end{bmatrix}, \quad \mathbf{A}\boldsymbol{\Sigma}_{\mathbf{X}}\mathbf{A}^T = \begin{bmatrix} 20 & 7 \\ 7 & 3 \end{bmatrix}.$$

Thus,

$$\text{Cov}(\mathbf{Y}) = \mathbf{A}\boldsymbol{\Sigma}_{\mathbf{X}}\mathbf{A}^T + \boldsymbol{\Sigma}_{\mathbf{Z}} = \begin{bmatrix} 21 & 7 \\ 7 & 5 \end{bmatrix}.$$

Final Results:

$$E[\mathbf{Y}] = \mathbf{0}, \quad \text{Cov}(\mathbf{Y}) = \boxed{\begin{bmatrix} 21 & 7 \\ 7 & 5 \end{bmatrix}}.$$